isabelle/BabElaborate.thy
@@ -1,0 +1,75 @@
+theory BabElaborate
+  imports IntRange ResolveTypedefs TypeEnv
+begin
+
+(* This "elaborates" a Babylon program by adding implicit casts, filling in missing type
+   annotations, etc, until the program is well-typed according to BabTypecheck.thy
+   (or an error is found).
+*)
+
+datatype TypeError =
+  TyErr_OutOfFuel Location
+  | TyErr_IntLiteralOutOfRange Location
+  | TyErr_InvalidCast Location
+  | TyErr_NegateRequiresSigned Location
+  | TyErr_ComplementRequiresFiniteInt Location
+  | TyErr_NotRequiresBool Location
+
+type_synonym Typedefs = "(string, DeclTypedef) fmap"
+
+(* Note: the type returned by elab_term is fully resolved (does not contain typedefs) *)
+fun elab_term :: "nat \<Rightarrow> Typedefs \<Rightarrow> GhostOrNot \<Rightarrow> BabTerm \<Rightarrow> TypeError list + (BabTerm \<times> BabType)"
+  where
+
+  (* Out of fuel case *)
+  "elab_term 0 _ _ tm = Inl [TyErr_OutOfFuel (bab_term_location tm)]"
+
+  (* Main case - valid fuel *)
+| "elab_term (Suc fuel) typedefs ghost tm =
+    (case tm of
+      BabTm_Literal loc lit \<Rightarrow>
+        (case lit of
+          BabLit_Bool b \<Rightarrow> Inr (tm, BabTy_Bool loc)
+        | BabLit_Int i \<Rightarrow>
+            (case get_type_for_int i of
+              Some (sign, bits) \<Rightarrow> Inr (tm, BabTy_FiniteInt loc sign bits)
+            | None \<Rightarrow> Inl [TyErr_IntLiteralOutOfRange loc])
+        | _ \<Rightarrow> undefined)  \<comment>\<open>TODO: other literals\<close>
+
+    | BabTm_Cast loc targetTy operand \<Rightarrow>
+        (case elab_term fuel typedefs ghost operand of
+          Inl errs \<Rightarrow> Inl errs
+        | Inr (newOperand, operandTy) \<Rightarrow>
+            (case resolve_typedefs fuel typedefs targetTy of 
+              None \<Rightarrow> Inl [TyErr_OutOfFuel (bab_type_location targetTy)]
+            | Some resolvedTargetTy \<Rightarrow>
+                if is_integer_type operandTy
+                \<and> is_integer_type resolvedTargetTy
+                \<and> (ghost = NotGhost \<longrightarrow> is_runtime_type resolvedTargetTy) then
+                    Inr (BabTm_Cast loc resolvedTargetTy newOperand, resolvedTargetTy)
+                else
+                    Inl [TyErr_InvalidCast loc]))
+
+    | BabTm_Unop loc op operand \<Rightarrow>
+        (case elab_term fuel typedefs ghost operand of
+          Inl errs \<Rightarrow> Inl errs
+        | Inr (newOperand, operandTy) \<Rightarrow>
+            (case op of
+              BabUnop_Negate \<Rightarrow>
+                if is_signed_integer_type operandTy then
+                  Inr (BabTm_Unop loc op newOperand, operandTy)
+                else
+                  Inl [TyErr_NegateRequiresSigned loc]
+            | BabUnop_Complement \<Rightarrow>
+                if is_finite_integer_type operandTy then
+                  Inr (BabTm_Unop loc op newOperand, operandTy)
+                else
+                  Inl [TyErr_ComplementRequiresFiniteInt loc]
+            | BabUnop_Not \<Rightarrow>
+                (case operandTy of
+                  BabTy_Bool _ \<Rightarrow> Inr (BabTm_Unop loc op newOperand, operandTy)
+                | _ \<Rightarrow> Inl [TyErr_NotRequiresBool loc])))
+
+    | _ \<Rightarrow> undefined)"  (* TODO: other cases *)
+
+end
