isabelle/BabTypecheck.thy
@@ -1,0 +1,161 @@
+theory BabTypecheck
+  imports TypeEnv IntRange
+begin
+
+(* This file defines type-correctness for an "elaborated" Babylon program, i.e. one in
+   which all typedefs have been expanded out, any necessary type inference has been 
+   performed, implicit casts have been inserted, etc. *)
+
+fun bab_term_type :: "BabTyEnv \<Rightarrow> GhostOrNot \<Rightarrow> BabTerm \<Rightarrow> BabType option"
+  where
+  (* Bool literals *)
+  "bab_term_type _ _ (BabTm_Literal loc (BabLit_Bool _)) = Some (BabTy_Bool loc)"
+
+  (* Int literals *)
+| "bab_term_type _ _ (BabTm_Literal loc (BabLit_Int i)) = 
+    (case get_type_for_int i of
+      Some (sign, bits) \<Rightarrow> Some (BabTy_FiniteInt loc sign bits)
+    | None \<Rightarrow> None)"
+
+  (* TODO: String and array literals *)
+
+  (* Cast *)
+| "bab_term_type env mode (BabTm_Cast loc target_ty operand) =
+    (case bab_term_type env mode operand of
+      None \<Rightarrow> None
+    | Some operand_ty \<Rightarrow>
+        if is_integer_type operand_ty
+        \<and> is_integer_type target_ty
+        \<and> (mode = NotGhost \<longrightarrow> is_runtime_type target_ty) then
+          Some target_ty
+        else
+          None)"
+
+  (* Unary operators - negate, complement, logical-not *)
+| "bab_term_type env mode (BabTm_Unop loc op operand) =
+    (case bab_term_type env mode operand of
+      Some operand_ty \<Rightarrow>
+        (case op of
+          BabUnop_Negate \<Rightarrow>
+            (if is_signed_integer_type operand_ty then Some operand_ty else None)
+        | BabUnop_Complement \<Rightarrow>
+            (if is_finite_integer_type operand_ty then Some operand_ty else None)
+        | BabUnop_Not \<Rightarrow>
+            (case operand_ty of BabTy_Bool _ \<Rightarrow> Some operand_ty | _ \<Rightarrow> None))
+    | None \<Rightarrow> None)"
+
+  (* If-then-else: condition must be bool, branches must have same type *)
+| "bab_term_type env mode (BabTm_If loc cond thenTm elseTm) =
+    (case (bab_term_type env mode cond,
+           bab_term_type env mode thenTm,
+           bab_term_type env mode elseTm) of
+      (Some (BabTy_Bool _), Some then_ty, Some else_ty) \<Rightarrow>
+        (if types_equal then_ty else_ty then Some then_ty else None)
+    | _ \<Rightarrow> None)"
+
+(* TODO: Other cases *)
+| "bab_term_type env mode _ = undefined"
+
+
+(* Runtime type invariant: If typechecking succeeds in NotGhost mode,
+   the resulting type must be runtime-compatible (no MathInt/MathReal) *)
+lemma bab_term_type_runtime_invariant:
+  assumes "bab_term_type env NotGhost tm = Some ty"
+  shows "is_runtime_type ty"
+using assms
+proof (induction env NotGhost tm arbitrary: ty rule: bab_term_type.induct)
+  case (1 uu loc uw)
+  (* BabTm_Literal loc (BabLit_Bool _) -> BabTy_Bool loc *)
+  then show ?case by auto
+next
+  case (2 ux loc i)
+  (* BabTm_Literal loc (BabLit_Int i) -> BabTy_FiniteInt *)
+  from "2.prems" show ?case
+    by (auto split: option.splits)
+next
+  case (3 env loc target_ty operand)
+  (* BabTm_Cast: guard requires is_runtime_type target_ty when mode = NotGhost *)
+  from "3.prems" show ?case
+    by (auto split: option.splits if_splits)
+next
+  case (4 env loc op operand)
+  (* BabTm_Unop: returns operand_ty which by IH is runtime type *)
+  from "4.prems" obtain operand_ty where
+    operand_typed: "bab_term_type env NotGhost operand = Some operand_ty"
+    by (auto split: option.splits)
+  hence "is_runtime_type operand_ty"
+    by (simp add: "4.hyps")
+  thus ?case
+    using "4.prems" operand_typed
+    by (auto split: option.splits if_splits BabType.splits BabUnop.splits)
+next
+  case (5 env loc cond thenTm elseTm)
+  (* BabTm_If: returns then_ty which by IH is runtime type *)
+  obtain cond_ty where cond_typed: "bab_term_type env NotGhost cond = Some cond_ty"
+    using "5.prems" by (auto split: option.splits)
+  obtain cond_loc where cond_bool: "cond_ty = BabTy_Bool cond_loc"
+    using "5.prems" cond_typed by (auto split: option.splits BabType.splits)
+  obtain then_ty where then_typed: "bab_term_type env NotGhost thenTm = Some then_ty"
+    using "5.prems" cond_typed cond_bool by (auto split: option.splits)
+  obtain else_ty where else_typed: "bab_term_type env NotGhost elseTm = Some else_ty"
+    using "5.prems" cond_typed cond_bool then_typed by (auto split: option.splits)
+  have result: "ty = then_ty"
+    using "5.prems" cond_typed cond_bool then_typed else_typed by (auto split: if_splits)
+  from then_typed have "is_runtime_type then_ty"
+    using "5.hyps"(2) cond_typed cond_bool by simp
+  thus ?case
+    using result by simp
+next
+  case ("6_1" env v vb)
+  then show ?case sorry
+next
+  case ("6_2" env v vb)
+  then show ?case sorry
+next
+  case ("6_3" env v va vb)
+  then show ?case sorry
+next
+  case ("6_4" env v va vb)
+  then show ?case sorry
+next
+  case ("6_5" env v va vb vc)
+  then show ?case sorry
+next
+  case ("6_6" env v va vb vc vd)
+  then show ?case sorry
+next
+  case ("6_7" env v va vb)
+  then show ?case sorry
+next
+  case ("6_8" env v va)
+  then show ?case sorry
+next
+  case ("6_9" env v va)
+  then show ?case sorry
+next
+  case ("6_10" env v va vb)
+  then show ?case sorry
+next
+  case ("6_11" env v va vb)
+  then show ?case sorry
+next
+  case ("6_12" env v va vb)
+  then show ?case sorry
+next
+  case ("6_13" env v va vb)
+  then show ?case sorry
+next
+  case ("6_14" env v va vb)
+  then show ?case sorry
+next
+  case ("6_15" env v va)
+  then show ?case sorry
+next
+  case ("6_16" env v va)
+  then show ?case sorry
+next
+  case ("6_17" env v va)
+  then show ?case sorry
+qed
+
+end
