isabelle/ConstEval.thy
@@ -1,0 +1,581 @@
+theory ConstEval
+  imports BabInterp
+begin
+
+(* Compile-time constant evaluation for array size expressions and similar.
+   This is used by the elaborator to convert BabDim_Fixed terms to BabDim_FixedInt. *)
+
+(* TODO: We can probably remove most of this and just call bab_interp_term instead.
+   After all, the correctness theorem below states that const_eval is basically the same
+   as bab_interp_term called in a suitable state - so we might as well just call bab_interp_term
+   directly! *)
+
+datatype ConstEvalError =
+  CEErr_NotConstant Location       (* Expression fundamentally cannot be a compile-time constant *)
+| CEErr_NotSupported Location      (* Expression could theoretically be const but we don't support it *)
+| CEErr_EvalFailed Location        (* Evaluation failed (div by zero, name not found, type error, etc.) *)
+
+(* Evaluate a compile-time constant expression.
+
+   Arguments:
+   - consts: Map from constant names to their values. The caller should remove any
+     names that are shadowed by local variables in the current scope.
+   - tm: The term to evaluate (should already be elaborated/type-checked)
+
+   Returns either an error or a BabValue.
+*)
+fun const_eval :: "(string, BabValue) fmap \<Rightarrow> BabTerm \<Rightarrow> ConstEvalError + BabValue"
+  and const_eval_binop :: "BabValue \<Rightarrow> (BabBinop \<times> BabTerm) list \<Rightarrow> (string, BabValue) fmap \<Rightarrow> Location \<Rightarrow> ConstEvalError + BabValue"
+where
+  (* Bool literal *)
+  "const_eval consts (BabTm_Literal _ (BabLit_Bool b)) = Inr (BV_Bool b)"
+
+  (* Int literal *)
+| "const_eval consts (BabTm_Literal loc (BabLit_Int i)) =
+    (case infer_literal_type i of
+      Some (sign, bits) \<Rightarrow> Inr (BV_FiniteInt sign bits i)
+    | None \<Rightarrow> Inl (CEErr_EvalFailed loc))"
+
+  (* String and array literals not supported *)
+| "const_eval consts (BabTm_Literal loc (BabLit_String _)) = Inl (CEErr_NotSupported loc)"
+| "const_eval consts (BabTm_Literal loc (BabLit_Array _)) = Inl (CEErr_NotSupported loc)"
+
+  (* Name lookup - only in constants map *)
+| "const_eval consts (BabTm_Name loc name _) =
+    (case fmlookup consts name of
+      Some v \<Rightarrow> Inr v
+    | None \<Rightarrow> Inl (CEErr_EvalFailed loc))"
+
+  (* Cast *)
+| "const_eval consts (BabTm_Cast loc targetTy operand) =
+    (case const_eval consts operand of
+      Inl err \<Rightarrow> Inl err
+    | Inr (BV_FiniteInt _ _ i) \<Rightarrow>
+        (case targetTy of
+          BabTy_FiniteInt _ tgt_sign tgt_bits \<Rightarrow>
+            if int_fits tgt_sign tgt_bits i
+            then Inr (BV_FiniteInt tgt_sign tgt_bits i)
+            else Inl (CEErr_EvalFailed loc)
+        | _ \<Rightarrow> Inl (CEErr_EvalFailed loc))
+    | Inr _ \<Rightarrow> Inl (CEErr_EvalFailed loc))"
+
+  (* If-then-else *)
+| "const_eval consts (BabTm_If loc cond thenTm elseTm) =
+    (case const_eval consts cond of
+      Inl err \<Rightarrow> Inl err
+    | Inr (BV_Bool True) \<Rightarrow> const_eval consts thenTm
+    | Inr (BV_Bool False) \<Rightarrow> const_eval consts elseTm
+    | Inr _ \<Rightarrow> Inl (CEErr_EvalFailed loc))"
+
+  (* Unary operators *)
+| "const_eval consts (BabTm_Unop loc BabUnop_Negate operand) =
+    (case const_eval consts operand of
+      Inr (BV_FiniteInt sign bits i) \<Rightarrow>
+        (let result = -i in
+         if int_fits sign bits result then Inr (BV_FiniteInt sign bits result)
+         else Inl (CEErr_EvalFailed loc))
+    | Inr _ \<Rightarrow> Inl (CEErr_EvalFailed loc)
+    | Inl err \<Rightarrow> Inl err)"
+
+| "const_eval consts (BabTm_Unop loc BabUnop_Complement operand) =
+    (case const_eval consts operand of
+      Inr (BV_FiniteInt sign bits i) \<Rightarrow>
+        Inr (BV_FiniteInt sign bits (int_complement sign bits i))
+    | Inr _ \<Rightarrow> Inl (CEErr_EvalFailed loc)
+    | Inl err \<Rightarrow> Inl err)"
+
+| "const_eval consts (BabTm_Unop loc BabUnop_Not operand) =
+    (case const_eval consts operand of
+      Inr (BV_Bool b) \<Rightarrow> Inr (BV_Bool (\<not>b))
+    | Inr _ \<Rightarrow> Inl (CEErr_EvalFailed loc)
+    | Inl err \<Rightarrow> Inl err)"
+
+  (* Binary operators *)
+| "const_eval consts (BabTm_Binop loc tm1 ops) =
+    (case const_eval consts tm1 of
+      Inr v1 \<Rightarrow> const_eval_binop v1 ops consts loc
+    | Inl err \<Rightarrow> Inl err)"
+
+  (* Tuple projection *)
+| "const_eval consts (BabTm_TupleProj loc tm idx) =
+    (case const_eval consts tm of
+      Inr (BV_Tuple vals) \<Rightarrow>
+        if idx < length vals then Inr (vals ! idx)
+        else Inl (CEErr_EvalFailed loc)
+    | Inr _ \<Rightarrow> Inl (CEErr_EvalFailed loc)
+    | Inl err \<Rightarrow> Inl err)"
+
+  (* Record projection *)
+| "const_eval consts (BabTm_RecordProj loc tm fieldName) =
+    (case const_eval consts tm of
+      Inr (BV_Record flds) \<Rightarrow>
+        (case map_of flds fieldName of
+          Some v \<Rightarrow> Inr v
+        | None \<Rightarrow> Inl (CEErr_EvalFailed loc))
+    | Inr _ \<Rightarrow> Inl (CEErr_EvalFailed loc)
+    | Inl err \<Rightarrow> Inl err)"
+
+  (* Things that are fundamentally not compile-time constants *)
+| "const_eval consts (BabTm_Quantifier loc _ _ _ _) = Inl (CEErr_NotConstant loc)"
+| "const_eval consts (BabTm_Call loc _ _) = Inl (CEErr_NotConstant loc)"
+| "const_eval consts (BabTm_Allocated loc _) = Inl (CEErr_NotConstant loc)"
+| "const_eval consts (BabTm_Old loc _) = Inl (CEErr_NotConstant loc)"
+
+  (* Things we could support but don't *)
+| "const_eval consts (BabTm_Let loc _ _ _) = Inl (CEErr_NotSupported loc)"
+| "const_eval consts (BabTm_Tuple loc _) = Inl (CEErr_NotSupported loc)"
+| "const_eval consts (BabTm_Record loc _) = Inl (CEErr_NotSupported loc)"
+| "const_eval consts (BabTm_RecordUpdate loc _ _) = Inl (CEErr_NotSupported loc)"
+| "const_eval consts (BabTm_ArrayProj loc _ _) = Inl (CEErr_NotSupported loc)"
+| "const_eval consts (BabTm_Match loc _ _) = Inl (CEErr_NotSupported loc)"
+| "const_eval consts (BabTm_Sizeof loc _) = Inl (CEErr_NotSupported loc)"
+
+  (* Binary operator chain evaluation *)
+| "const_eval_binop v1 [] _ _ = Inr v1"
+| "const_eval_binop v1 ((op, tm2) # rest) consts loc =
+    (case const_eval consts tm2 of
+      Inr v2 \<Rightarrow>
+        (case eval_binop op v1 v2 of
+          BIR_Success result \<Rightarrow> const_eval_binop result rest consts loc
+        | _ \<Rightarrow> Inl (CEErr_EvalFailed loc))
+    | Inl err \<Rightarrow> Inl err)"
+
+(* Helper to evaluate an expression and extract a u64 integer (for array sizes) *)
+fun const_eval_to_u64 :: "(string, BabValue) fmap \<Rightarrow> BabTerm \<Rightarrow> ConstEvalError + int" where
+  "const_eval_to_u64 consts tm =
+    (case const_eval consts tm of
+      Inr (BV_FiniteInt Unsigned IntBits_64 n) \<Rightarrow> Inr n
+    | Inr _ \<Rightarrow> Inl (CEErr_EvalFailed (bab_term_location tm))
+    | Inl err \<Rightarrow> Inl err)"
+
+
+(* ========== Correctness theorem ========== *)
+
+(* A state is suitable for const evaluation if it has no locals/refs and
+   constants match the provided map *)
+definition const_eval_state :: "(string, BabValue) fmap \<Rightarrow> 'w BabState \<Rightarrow> bool" where
+  "const_eval_state consts state \<equiv>
+     BS_Constants state = consts \<and>
+     BS_Locals state = fmempty \<and>
+     BS_RefVars state = fmempty"
+
+(* Main correctness theorem using the induction principle generated for const_eval.
+
+   This shows that if const_eval and/or const_eval_binop succeed, then the interpreter
+   (in an appropriate state) would also have succeeded obtaining the same value (or run
+   out of fuel). In other words, const_eval is "sound", but not necessarily "complete" 
+   (i.e. there exist runtime-only expressions that cannot be evaluated at compile time).
+
+   A subtle point: We don't rule out that the constant evaluator might succeed on an
+   expression that actually diverges at runtime (i.e. runs out of fuel in the interpreter
+   for every fuel value). But this is not a realistic possibility because the constant
+   evaluator doesn't support any construct (such as function calls or while-loops) that
+   might cause divergence.
+*)
+theorem const_eval_interp_correspondence:
+  assumes "const_eval_state constants state"
+  shows "\<forall>fuel v. const_eval constants tm = Inr v \<longrightarrow>
+            (interp_bab_term fuel state tm = BIR_Success v \<or>
+             interp_bab_term fuel state tm = BIR_InsufficientFuel)"
+    and "\<forall>fuel v. const_eval_binop v1 ops constants loc = Inr v \<longrightarrow>
+            (interp_bab_binop fuel state v1 ops = BIR_Success v \<or>
+             interp_bab_binop fuel state v1 ops = BIR_InsufficientFuel)"
+  using assms
+proof (induction rule: const_eval_const_eval_binop.induct)
+  (* Bool literal *)
+  case (1 constants loc b)
+  then show ?case
+    by (metis const_eval.simps(1) interp_bab_term.simps(1,2) not0_implies_Suc
+        sum.inject(2))
+next
+  (* Int literal *)
+  case (2 constants loc i)
+  show ?case
+  proof (intro allI impI)
+    fix fuel v
+    assume ce: "const_eval constants (BabTm_Literal loc (BabLit_Int i)) = Inr v"
+    show "interp_bab_term fuel state (BabTm_Literal loc (BabLit_Int i)) = BIR_Success v \<or>
+          interp_bab_term fuel state (BabTm_Literal loc (BabLit_Int i)) = BIR_InsufficientFuel"
+      using ce by (cases fuel; auto split: option.splits if_splits)
+  qed
+next
+  (* String literal - returns NotSupported error *)
+  case (3 constants loc uv)
+  then show ?case by simp
+next
+  (* Array literal - returns NotSupported error *)
+  case (4 constants loc uw)
+  then show ?case by simp
+next
+  (* Name lookup *)
+  case (5 constants loc name ux)
+  show ?case
+  proof (intro allI impI)
+    fix fuel v
+    assume ce: "const_eval constants (BabTm_Name loc name ux) = Inr v"
+    show "interp_bab_term fuel state (BabTm_Name loc name ux) = BIR_Success v \<or>
+          interp_bab_term fuel state (BabTm_Name loc name ux) = BIR_InsufficientFuel"
+      using ce "5.prems" by (cases fuel; auto simp: const_eval_state_def split: option.splits)
+  qed
+next
+  (* Cast *)
+  case (6 constants loc targetTy operand)
+  show ?case
+  proof (intro allI impI)
+    fix fuel v
+    assume ce: "const_eval constants (BabTm_Cast loc targetTy operand) = Inr v"
+    show "interp_bab_term fuel state (BabTm_Cast loc targetTy operand) = BIR_Success v \<or>
+          interp_bab_term fuel state (BabTm_Cast loc targetTy operand) = BIR_InsufficientFuel"
+    proof (cases fuel)
+      case 0 then show ?thesis by simp
+    next
+      case (Suc n)
+      from ce obtain src_sign src_bits i tgt_loc tgt_sign tgt_bits where
+        ce_op: "const_eval constants operand = Inr (BV_FiniteInt src_sign src_bits i)" and
+        tgt: "targetTy = BabTy_FiniteInt tgt_loc tgt_sign tgt_bits" and
+        fits: "int_fits tgt_sign tgt_bits i" and
+        v_eq: "v = BV_FiniteInt tgt_sign tgt_bits i"
+        by (auto split: sum.splits BabValue.splits BabType.splits if_splits)
+      from "6.IH"[OF "6.prems"] ce_op
+      have ih: "interp_bab_term n state operand = BIR_Success (BV_FiniteInt src_sign src_bits i) \<or>
+                interp_bab_term n state operand = BIR_InsufficientFuel" by auto
+      then show ?thesis
+      proof
+        assume "interp_bab_term n state operand = BIR_Success (BV_FiniteInt src_sign src_bits i)"
+        then show ?thesis using Suc tgt fits v_eq by simp
+      next
+        assume "interp_bab_term n state operand = BIR_InsufficientFuel"
+        then show ?thesis using Suc by simp
+      qed
+    qed
+  qed
+next
+  (* If-then-else *)
+  case (7 constants loc cond thenTm elseTm)
+  show ?case
+  proof (intro allI impI)
+    fix fuel v
+    assume ce: "const_eval constants (BabTm_If loc cond thenTm elseTm) = Inr v"
+    show "interp_bab_term fuel state (BabTm_If loc cond thenTm elseTm) = BIR_Success v \<or>
+          interp_bab_term fuel state (BabTm_If loc cond thenTm elseTm) = BIR_InsufficientFuel"
+    proof (cases fuel)
+      case 0 then show ?thesis by simp
+    next
+      case (Suc n)
+      from ce obtain b where
+        ce_cond: "const_eval constants cond = Inr (BV_Bool b)" and
+        ce_branch: "if b then const_eval constants thenTm = Inr v
+                    else const_eval constants elseTm = Inr v"
+        by (auto split: sum.splits BabValue.splits bool.splits)
+      from "7.IH"(1)[OF "7.prems"] ce_cond
+      have ih_cond: "interp_bab_term n state cond = BIR_Success (BV_Bool b) \<or>
+                     interp_bab_term n state cond = BIR_InsufficientFuel" by auto
+      show ?thesis
+      proof (cases b)
+        case True
+        with ce_branch have ce_then: "const_eval constants thenTm = Inr v" by simp
+        from "7.IH"(2) True ce_cond "7.prems" ce_then
+        have ih_then: "interp_bab_term n state thenTm = BIR_Success v \<or>
+                       interp_bab_term n state thenTm = BIR_InsufficientFuel" by auto
+        from ih_cond show ?thesis
+        proof
+          assume "interp_bab_term n state cond = BIR_Success (BV_Bool b)"
+          with ih_then Suc True show ?thesis by auto
+        next
+          assume "interp_bab_term n state cond = BIR_InsufficientFuel"
+          then show ?thesis using Suc by simp
+        qed
+      next
+        case False
+        with ce_branch have ce_else: "const_eval constants elseTm = Inr v" by simp
+        from "7.IH"(3) False ce_cond "7.prems" ce_else
+        have ih_else: "interp_bab_term n state elseTm = BIR_Success v \<or>
+                       interp_bab_term n state elseTm = BIR_InsufficientFuel" by auto
+        from ih_cond show ?thesis
+        proof
+          assume "interp_bab_term n state cond = BIR_Success (BV_Bool b)"
+          with ih_else Suc False show ?thesis by auto
+        next
+          assume "interp_bab_term n state cond = BIR_InsufficientFuel"
+          then show ?thesis using Suc by simp
+        qed
+      qed
+    qed
+  qed
+next
+  (* Unop Negate *)
+  case (8 constants loc operand)
+  show ?case
+  proof (intro allI impI)
+    fix fuel v
+    assume ce: "const_eval constants (BabTm_Unop loc BabUnop_Negate operand) = Inr v"
+    show "interp_bab_term fuel state (BabTm_Unop loc BabUnop_Negate operand) = BIR_Success v \<or>
+          interp_bab_term fuel state (BabTm_Unop loc BabUnop_Negate operand) = BIR_InsufficientFuel"
+    proof (cases fuel)
+      case 0 then show ?thesis by simp
+    next
+      case (Suc n)
+      from ce obtain sign bits i where
+        ce_op: "const_eval constants operand = Inr (BV_FiniteInt sign bits i)" and
+        fits: "int_fits sign bits (-i)" and
+        v_eq: "v = BV_FiniteInt sign bits (-i)"
+        by (auto split: sum.splits BabValue.splits if_splits simp: Let_def)
+      from "8.IH"[OF "8.prems"] ce_op
+      have ih: "interp_bab_term n state operand = BIR_Success (BV_FiniteInt sign bits i) \<or>
+                interp_bab_term n state operand = BIR_InsufficientFuel" by auto
+      then show ?thesis
+      proof
+        assume "interp_bab_term n state operand = BIR_Success (BV_FiniteInt sign bits i)"
+        then show ?thesis using Suc fits v_eq by (simp add: Let_def)
+      next
+        assume "interp_bab_term n state operand = BIR_InsufficientFuel"
+        then show ?thesis using Suc by simp
+      qed
+    qed
+  qed
+next
+  (* Unop Complement *)
+  case (9 constants loc operand)
+  show ?case
+  proof (intro allI impI)
+    fix fuel v
+    assume ce: "const_eval constants (BabTm_Unop loc BabUnop_Complement operand) = Inr v"
+    show "interp_bab_term fuel state (BabTm_Unop loc BabUnop_Complement operand) = BIR_Success v \<or>
+          interp_bab_term fuel state (BabTm_Unop loc BabUnop_Complement operand) = BIR_InsufficientFuel"
+    proof (cases fuel)
+      case 0 then show ?thesis by simp
+    next
+      case (Suc n)
+      from ce obtain sign bits i where
+        ce_op: "const_eval constants operand = Inr (BV_FiniteInt sign bits i)" and
+        v_eq: "v = BV_FiniteInt sign bits (int_complement sign bits i)"
+        by (auto split: sum.splits BabValue.splits)
+      from "9.IH"[OF "9.prems"] ce_op
+      have ih: "interp_bab_term n state operand = BIR_Success (BV_FiniteInt sign bits i) \<or>
+                interp_bab_term n state operand = BIR_InsufficientFuel" by auto
+      then show ?thesis
+      proof
+        assume "interp_bab_term n state operand = BIR_Success (BV_FiniteInt sign bits i)"
+        then show ?thesis using Suc v_eq by simp
+      next
+        assume "interp_bab_term n state operand = BIR_InsufficientFuel"
+        then show ?thesis using Suc by simp
+      qed
+    qed
+  qed
+next
+  (* Unop Not *)
+  case (10 constants loc operand)
+  show ?case
+  proof (intro allI impI)
+    fix fuel v
+    assume ce: "const_eval constants (BabTm_Unop loc BabUnop_Not operand) = Inr v"
+    show "interp_bab_term fuel state (BabTm_Unop loc BabUnop_Not operand) = BIR_Success v \<or>
+          interp_bab_term fuel state (BabTm_Unop loc BabUnop_Not operand) = BIR_InsufficientFuel"
+    proof (cases fuel)
+      case 0 then show ?thesis by simp
+    next
+      case (Suc n)
+      from ce obtain b where
+        ce_op: "const_eval constants operand = Inr (BV_Bool b)" and
+        v_eq: "v = BV_Bool (\<not>b)"
+        by (auto split: sum.splits BabValue.splits)
+      from "10.IH"[OF "10.prems"] ce_op
+      have ih: "interp_bab_term n state operand = BIR_Success (BV_Bool b) \<or>
+                interp_bab_term n state operand = BIR_InsufficientFuel" by auto
+      then show ?thesis
+      proof
+        assume "interp_bab_term n state operand = BIR_Success (BV_Bool b)"
+        then show ?thesis using Suc v_eq by simp
+      next
+        assume "interp_bab_term n state operand = BIR_InsufficientFuel"
+        then show ?thesis using Suc by simp
+      qed
+    qed
+  qed
+next
+  (* Binop *)
+  case (11 constants loc tm1 ops)
+  show ?case
+  proof (intro allI impI)
+    fix fuel v
+    assume ce: "const_eval constants (BabTm_Binop loc tm1 ops) = Inr v"
+    show "interp_bab_term fuel state (BabTm_Binop loc tm1 ops) = BIR_Success v \<or>
+          interp_bab_term fuel state (BabTm_Binop loc tm1 ops) = BIR_InsufficientFuel"
+    proof (cases fuel)
+      case 0 then show ?thesis by simp
+    next
+      case (Suc n)
+      from ce obtain v1' where
+        ce_tm1: "const_eval constants tm1 = Inr v1'" and
+        ce_ops: "const_eval_binop v1' ops constants loc = Inr v"
+        by (auto split: sum.splits)
+      from "11.IH"(1)[OF "11.prems"] ce_tm1
+      have ih_tm1: "interp_bab_term n state tm1 = BIR_Success v1' \<or>
+                    interp_bab_term n state tm1 = BIR_InsufficientFuel" by auto
+      from "11.IH"(2)[OF ce_tm1 "11.prems"] ce_ops
+      have ih_ops: "interp_bab_binop n state v1' ops = BIR_Success v \<or>
+                    interp_bab_binop n state v1' ops = BIR_InsufficientFuel" by auto
+      from ih_tm1 show ?thesis
+      proof
+        assume "interp_bab_term n state tm1 = BIR_Success v1'"
+        with ih_ops Suc show ?thesis by auto
+      next
+        assume "interp_bab_term n state tm1 = BIR_InsufficientFuel"
+        then show ?thesis using Suc by simp
+      qed
+    qed
+  qed
+next
+  (* TupleProj *)
+  case (12 constants loc tm idx)
+  show ?case
+  proof (intro allI impI)
+    fix fuel v
+    assume ce: "const_eval constants (BabTm_TupleProj loc tm idx) = Inr v"
+    show "interp_bab_term fuel state (BabTm_TupleProj loc tm idx) = BIR_Success v \<or>
+          interp_bab_term fuel state (BabTm_TupleProj loc tm idx) = BIR_InsufficientFuel"
+    proof (cases fuel)
+      case 0 then show ?thesis by simp
+    next
+      case (Suc n)
+      from ce obtain vals where
+        ce_tm: "const_eval constants tm = Inr (BV_Tuple vals)" and
+        idx_ok: "idx < length vals" and
+        v_eq: "v = vals ! idx"
+        by (auto split: sum.splits BabValue.splits if_splits)
+      from "12.IH"[OF "12.prems"] ce_tm
+      have ih: "interp_bab_term n state tm = BIR_Success (BV_Tuple vals) \<or>
+                interp_bab_term n state tm = BIR_InsufficientFuel" by auto
+      then show ?thesis
+      proof
+        assume "interp_bab_term n state tm = BIR_Success (BV_Tuple vals)"
+        then show ?thesis using Suc idx_ok v_eq by simp
+      next
+        assume "interp_bab_term n state tm = BIR_InsufficientFuel"
+        then show ?thesis using Suc by simp
+      qed
+    qed
+  qed
+next
+  (* RecordProj *)
+  case (13 constants loc tm fieldName)
+  show ?case
+  proof (intro allI impI)
+    fix fuel v
+    assume ce: "const_eval constants (BabTm_RecordProj loc tm fieldName) = Inr v"
+    show "interp_bab_term fuel state (BabTm_RecordProj loc tm fieldName) = BIR_Success v \<or>
+          interp_bab_term fuel state (BabTm_RecordProj loc tm fieldName) = BIR_InsufficientFuel"
+    proof (cases fuel)
+      case 0 then show ?thesis by simp
+    next
+      case (Suc n)
+      from ce obtain flds where
+        ce_tm: "const_eval constants tm = Inr (BV_Record flds)" and
+        lookup: "map_of flds fieldName = Some v"
+        by (auto split: sum.splits BabValue.splits option.splits)
+      from "13.IH"[OF "13.prems"] ce_tm
+      have ih: "interp_bab_term n state tm = BIR_Success (BV_Record flds) \<or>
+                interp_bab_term n state tm = BIR_InsufficientFuel" by auto
+      then show ?thesis
+      proof
+        assume "interp_bab_term n state tm = BIR_Success (BV_Record flds)"
+        then show ?thesis using Suc lookup by simp
+      next
+        assume "interp_bab_term n state tm = BIR_InsufficientFuel"
+        then show ?thesis using Suc by simp
+      qed
+    qed
+  qed
+next
+  (* Quantifier - returns NotConstant error *)
+  case (14 constants loc uy uz va vb)
+  then show ?case by simp
+next
+  (* Call - returns NotConstant error *)
+  case (15 constants loc vc vd)
+  then show ?case by simp
+next
+  (* Allocated - returns NotConstant error *)
+  case (16 constants loc ve)
+  then show ?case by simp
+next
+  (* Old - returns NotConstant error *)
+  case (17 constants loc vf)
+  then show ?case by simp
+next
+  (* Let - returns NotSupported error *)
+  case (18 constants loc vg vh vi)
+  then show ?case by simp
+next
+  (* Tuple - returns NotSupported error *)
+  case (19 constants loc vj)
+  then show ?case by simp
+next
+  (* Record - returns NotSupported error *)
+  case (20 constants loc vk)
+  then show ?case by simp
+next
+  (* RecordUpdate - returns NotSupported error *)
+  case (21 constants loc vl vm)
+  then show ?case by simp
+next
+  (* ArrayProj - returns NotSupported error *)
+  case (22 constants loc vn vo)
+  then show ?case by simp
+next
+  (* Match - returns NotSupported error *)
+  case (23 constants loc vp vq)
+  then show ?case by simp
+next
+  (* Sizeof - returns NotSupported error *)
+  case (24 constants loc vr)
+  then show ?case by simp
+next
+  (* Binop chain - empty list *)
+  case (25 v1 vs vt)
+  then show ?case
+    by (metis const_eval_binop.simps(1) interp_bab_binop.simps(1,2) nat.exhaust_sel
+        sum.inject(2))
+next
+  (* Binop chain - cons *)
+  case (26 v1 op tm2 rest constants loc)
+  show ?case
+  proof (intro allI impI)
+    fix fuel v
+    assume ce: "const_eval_binop v1 ((op, tm2) # rest) constants loc = Inr v"
+    show "interp_bab_binop fuel state v1 ((op, tm2) # rest) = BIR_Success v \<or>
+          interp_bab_binop fuel state v1 ((op, tm2) # rest) = BIR_InsufficientFuel"
+    proof (cases fuel)
+      case 0 then show ?thesis by simp
+    next
+      case (Suc n)
+      from ce obtain v2 intermediate where
+        ce_tm2: "const_eval constants tm2 = Inr v2" and
+        eval_op: "eval_binop op v1 v2 = BIR_Success intermediate" and
+        ce_rest: "const_eval_binop intermediate rest constants loc = Inr v"
+        by (auto split: sum.splits BabInterpResult.splits)
+      from "26.IH"(1)[OF "26.prems"] ce_tm2
+      have ih_tm2: "interp_bab_term n state tm2 = BIR_Success v2 \<or>
+                    interp_bab_term n state tm2 = BIR_InsufficientFuel" by auto
+      from "26.IH"(2) ce_tm2 refl eval_op "26.prems" ce_rest
+      have ih_rest: "interp_bab_binop n state intermediate rest = BIR_Success v \<or>
+                     interp_bab_binop n state intermediate rest = BIR_InsufficientFuel" by auto
+      from ih_tm2 show ?thesis
+      proof
+        assume tm2_succ: "interp_bab_term n state tm2 = BIR_Success v2"
+        from ih_rest show ?thesis
+        proof
+          assume "interp_bab_binop n state intermediate rest = BIR_Success v"
+          then show ?thesis using Suc tm2_succ eval_op by simp
+        next
+          assume "interp_bab_binop n state intermediate rest = BIR_InsufficientFuel"
+          then show ?thesis using Suc tm2_succ eval_op by simp
+        qed
+      next
+        assume "interp_bab_term n state tm2 = BIR_InsufficientFuel"
+        then show ?thesis using Suc by simp
+      qed
+    qed
+  qed
+qed
