isabelle/ResolveTypedefs.thy
@@ -1,0 +1,580 @@
+theory ResolveTypedefs
+  imports BabSyntax
+begin
+
+(* Resolve a typedef name to its underlying type *)
+(* This recursively resolves all typedefs found inside e.g. tuples and arrays as well *)
+(* Returns None if fuel runs out, Some ty otherwise *)
+fun resolve_typedefs :: "nat \<Rightarrow> (string, DeclTypedef) fmap \<Rightarrow> BabType \<Rightarrow> BabType option" where
+  "resolve_typedefs 0 _ _ = None"  (* Fuel exhausted *)
+| "resolve_typedefs (Suc fuel) typedefs (BabTy_Name loc name tyargs) =
+    (case those (map (resolve_typedefs fuel typedefs) tyargs) of
+      None \<Rightarrow> None
+    | Some resolved_tyargs \<Rightarrow>
+        (case fmlookup typedefs name of
+          Some typedef \<Rightarrow>
+            (case DT_Definition typedef of
+              Some body \<Rightarrow>
+                let typarams = DT_TyArgs typedef;
+                    subst = fmap_of_list (zip typarams resolved_tyargs)
+                in resolve_typedefs fuel typedefs (substitute_bab_type subst body)
+            | None \<Rightarrow>
+                Some (BabTy_Name loc name resolved_tyargs))
+        | None \<Rightarrow>
+            Some (BabTy_Name loc name resolved_tyargs)))"
+| "resolve_typedefs (Suc fuel) typedefs (BabTy_Tuple loc tys) =
+    (case those (map (resolve_typedefs fuel typedefs) tys) of
+      None \<Rightarrow> None
+    | Some resolved_tys \<Rightarrow> Some (BabTy_Tuple loc resolved_tys))"
+| "resolve_typedefs (Suc fuel) typedefs (BabTy_Record loc flds) =
+    (case those (map (\<lambda>(name, ty). case resolve_typedefs fuel typedefs ty of
+                                     None \<Rightarrow> None
+                                   | Some rty \<Rightarrow> Some (name, rty)) flds) of
+      None \<Rightarrow> None
+    | Some resolved_flds \<Rightarrow> Some (BabTy_Record loc resolved_flds))"
+| "resolve_typedefs (Suc fuel) typedefs (BabTy_Array loc ty dims) =
+    (case resolve_typedefs fuel typedefs ty of
+      None \<Rightarrow> None
+    | Some resolved_ty \<Rightarrow> Some (BabTy_Array loc resolved_ty dims))"
+| "resolve_typedefs (Suc fuel) _ ty = Some ty"  (* Base types *)
+
+
+(* Helper lemma: if those succeeds on a list, every element is Some *)
+lemma those_Some_implies_all_Some:
+  assumes "those xs = Some ys"
+  shows "\<forall>x \<in> set xs. x \<noteq> None"
+  using assms
+  by (induction xs arbitrary: ys) (auto split: option.splits)
+
+(* Helper lemma: those preserves length *)
+lemma those_length:
+  assumes "those xs = Some ys"
+  shows "length ys = length xs"
+  using assms
+  by (induction xs arbitrary: ys) (auto split: option.splits)
+
+(* Helper lemma: those nth element *)
+lemma those_nth:
+  assumes "those xs = Some ys" and "i < length xs"
+  shows "xs ! i = Some (ys ! i)"
+  using assms
+proof (induction xs arbitrary: ys i)
+  case Nil
+  then show ?case by simp
+next
+  case (Cons x xs)
+  from Cons.prems obtain y ys' where "x = Some y" and "those xs = Some ys'" and "ys = y # ys'"
+    by (auto split: option.splits)
+  show ?case
+  proof (cases i)
+    case 0
+    with \<open>x = Some y\<close> \<open>ys = y # ys'\<close> show ?thesis by simp
+  next
+    case (Suc j)
+    with Cons.prems have "j < length xs" by simp
+    with Cons.IH \<open>those xs = Some ys'\<close> have "xs ! j = Some (ys' ! j)" by simp
+    with Suc \<open>ys = y # ys'\<close> show ?thesis by simp
+  qed
+qed
+
+(* Helper lemma: those iff all elements are Some *)
+lemma those_iff_all_Some:
+  "those xs = Some ys \<longleftrightarrow> (length ys = length xs \<and> (\<forall>i < length xs. xs ! i = Some (ys ! i)))"
+proof
+  assume "those xs = Some ys"
+  then show "length ys = length xs \<and> (\<forall>i<length xs. xs ! i = Some (ys ! i))"
+    using those_length those_nth by blast
+next
+  assume "length ys = length xs \<and> (\<forall>i<length xs. xs ! i = Some (ys ! i))"
+  then show "those xs = Some ys"
+  proof (induction xs arbitrary: ys)
+    case Nil
+    then show ?case by simp
+  next
+    case (Cons x xs)
+    then obtain y ys' where "ys = y # ys'" by (cases ys) auto
+    with Cons have "x = Some y" by (metis length_Cons nth_Cons_0 zero_less_Suc)
+    moreover from Cons \<open>ys = y # ys'\<close> have "length ys' = length xs" by simp
+    moreover from Cons \<open>ys = y # ys'\<close> have "\<forall>i<length xs. xs ! i = Some (ys' ! i)"
+      by (metis Suc_less_eq length_Cons nth_Cons_Suc)
+    ultimately show ?case using Cons.IH \<open>ys = y # ys'\<close> by auto
+  qed
+qed
+
+(* Helper lemma: map f xs = ys iff they have same length and agree pointwise *)
+lemma map_nth_eq_conv:
+  "map f xs = ys \<longleftrightarrow> (length ys = length xs \<and> (\<forall>i < length xs. f (xs ! i) = ys ! i))"
+  by (auto simp: list_eq_iff_nth_eq)
+
+
+(* resolve_typedefs is monotonic in fuel *)
+lemma resolve_typedefs_monotonic:
+  assumes "resolve_typedefs fuel typedefs ty = Some ty'"
+    and "fuel' \<ge> fuel"
+  shows "resolve_typedefs fuel' typedefs ty = Some ty'"
+  using assms
+proof (induction fuel typedefs ty arbitrary: fuel' ty' rule: resolve_typedefs.induct)
+  case (1 typedefs ty)
+  (* fuel = 0 case *)
+  then show ?case by simp
+next
+  case (2 fuel typedefs loc name tyargs)
+  (* BabTy_Name case *)
+  show ?case
+  proof (cases fuel')
+    case 0
+    with 2 show ?thesis by simp
+  next
+    case (Suc fuel'_pred)
+    with 2 have fuel_le: "fuel'_pred \<ge> fuel" by simp
+
+    (* Extract what we know from the assumption *)
+    from 2 have "resolve_typedefs (Suc fuel) typedefs (BabTy_Name loc name tyargs) = Some ty'"
+      by blast
+    then obtain resolved_tyargs where
+      tyargs_resolved: "those (map (resolve_typedefs fuel typedefs) tyargs) = Some resolved_tyargs"
+      by (auto split: option.splits)
+
+    (* Use IH to show tyargs resolve the same with more fuel *)
+    have ih_tyargs: "\<forall>t \<in> set tyargs. \<forall>ty_t.
+          resolve_typedefs fuel typedefs t = Some ty_t \<longrightarrow>
+          resolve_typedefs fuel'_pred typedefs t = Some ty_t"
+      using "2.IH" fuel_le by blast
+
+    (* Show that map with fuel'_pred gives same result as map with fuel *)
+    have all_some: "\<forall>t \<in> set (map (resolve_typedefs fuel typedefs) tyargs). t \<noteq> None"
+      using tyargs_resolved those_Some_implies_all_Some by metis
+
+    have tyargs_eq: "\<forall>t \<in> set tyargs. resolve_typedefs fuel'_pred typedefs t = resolve_typedefs fuel typedefs t"
+    proof
+      fix t
+      assume t_in: "t \<in> set tyargs"
+      then have "resolve_typedefs fuel typedefs t \<in> set (map (resolve_typedefs fuel typedefs) tyargs)"
+        by auto
+      with all_some have "resolve_typedefs fuel typedefs t \<noteq> None"
+        by auto
+      then obtain ty_t where res_fuel: "resolve_typedefs fuel typedefs t = Some ty_t"
+        by auto
+      with t_in ih_tyargs have "resolve_typedefs fuel'_pred typedefs t = Some ty_t"
+        by blast
+      with res_fuel show "resolve_typedefs fuel'_pred typedefs t = resolve_typedefs fuel typedefs t"
+        by simp
+    qed
+
+    have tyargs_resolved': "those (map (resolve_typedefs fuel'_pred typedefs) tyargs) = Some resolved_tyargs"
+      using tyargs_eq tyargs_resolved map_ext by metis
+
+    (* Now handle the typedef lookup and body substitution *)
+    show ?thesis
+    proof (cases "fmlookup typedefs name")
+      case None
+      (* No typedef found - just return Name with resolved tyargs *)
+      from 2 None tyargs_resolved have "ty' = BabTy_Name loc name resolved_tyargs"
+        by auto
+      with None tyargs_resolved' Suc show ?thesis by auto
+    next
+      case SomeTydef: (Some tydef)
+      then show ?thesis
+      proof (cases "DT_Definition tydef")
+        case None
+        (* Abstract/extern type - just return Name with resolved tyargs *)
+        with SomeTydef tyargs_resolved tyargs_resolved' Suc show ?thesis
+          using "2.prems"(1) by force 
+      next
+        case SomeBody: (Some body)
+        (* Concrete typedef - need to substitute and recurse *)
+        define typarams where "typarams = DT_TyArgs tydef"
+        define subst where "subst = fmap_of_list (zip typarams resolved_tyargs)"
+        define subst_body where "subst_body = substitute_bab_type subst body"
+
+        from 2 SomeTydef SomeBody tyargs_resolved have
+          "resolve_typedefs fuel typedefs subst_body = Some ty'"
+          by (metis (no_types, lifting) option.simps(5) resolve_typedefs.simps(2) subst_body_def subst_def
+              typarams_def)
+
+        (* Use the IH for the substituted body *)
+        with fuel_le "2.IH" have
+          "resolve_typedefs fuel'_pred typedefs subst_body = Some ty'"
+          using SomeBody SomeTydef subst_body_def subst_def tyargs_resolved typarams_def by blast
+          
+        with tyargs_resolved' SomeTydef SomeBody Suc show ?thesis
+          by (auto simp: typarams_def subst_def subst_body_def)
+      qed
+    qed
+  qed
+next
+  case (3 fuel typedefs loc tys)
+  (* BabTy_Tuple case *)
+  show ?case
+  proof (cases fuel')
+    case 0
+    with 3 show ?thesis by simp
+  next
+    case (Suc fuel'_pred)
+    with 3 have fuel_le: "fuel \<le> fuel'_pred" by simp
+    from 3 obtain resolved_tys where
+      those_result: "those (map (resolve_typedefs fuel typedefs) tys) = Some resolved_tys"
+      and ty'_eq: "ty' = BabTy_Tuple loc resolved_tys"
+      by (auto split: option.splits)
+
+    (* Use IH for each element of tys *)
+    have ih_all: "\<forall>t \<in> set tys. \<forall>ty_t.
+          resolve_typedefs fuel typedefs t = Some ty_t \<longrightarrow>
+          resolve_typedefs fuel'_pred typedefs t = Some ty_t"
+      using "3.IH" fuel_le by blast
+
+    (* Show that map with fuel'_pred gives same result as map with fuel *)
+    have all_some: "\<forall>t \<in> set (map (resolve_typedefs fuel typedefs) tys). t \<noteq> None"
+      using those_result those_Some_implies_all_Some
+      by metis 
+
+    have map_eq: "\<forall>t \<in> set tys. resolve_typedefs fuel'_pred typedefs t = resolve_typedefs fuel typedefs t"
+    proof
+      fix t
+      assume t_in: "t \<in> set tys"
+      then have "resolve_typedefs fuel typedefs t \<in> set (map (resolve_typedefs fuel typedefs) tys)"
+        by auto
+      with all_some have "resolve_typedefs fuel typedefs t \<noteq> None"
+        by auto
+      then obtain ty_t where res_fuel: "resolve_typedefs fuel typedefs t = Some ty_t"
+        by auto
+      with t_in ih_all have "resolve_typedefs fuel'_pred typedefs t = Some ty_t"
+        by blast
+      with res_fuel show "resolve_typedefs fuel'_pred typedefs t = resolve_typedefs fuel typedefs t"
+        by simp
+    qed
+
+    have "those (map (resolve_typedefs fuel'_pred typedefs) tys) = those (map (resolve_typedefs fuel typedefs) tys)"
+      using map_eq map_ext by metis
+    with those_result have "those (map (resolve_typedefs fuel'_pred typedefs) tys) = Some resolved_tys"
+      by simp
+
+    with Suc ty'_eq show ?thesis by simp
+  qed
+next
+  case (4 fuel typedefs loc flds)
+  (* BabTy_Record case *)
+  show ?case
+  proof (cases fuel')
+    case 0
+    with 4 show ?thesis by simp
+  next
+    case (Suc fuel'_pred)
+    with 4 have fuel_le: "fuel \<le> fuel'_pred" by simp
+    from 4 obtain resolved_flds where
+      those_result: "those (map (\<lambda>(name, ty). case resolve_typedefs fuel typedefs ty of
+                                     None \<Rightarrow> None
+                                   | Some rty \<Rightarrow> Some (name, rty)) flds) = Some resolved_flds"
+      and ty'_eq: "ty' = BabTy_Record loc resolved_flds"
+      by (auto split: option.splits)
+
+    (* Use IH for each field type *)
+    have ih_all: "\<forall>(name, ty) \<in> set flds. \<forall>ty_t.
+          resolve_typedefs fuel typedefs ty = Some ty_t \<longrightarrow>
+          resolve_typedefs fuel'_pred typedefs ty = Some ty_t"
+      using "4.IH" fuel_le by blast
+
+    (* Show that map with fuel'_pred gives same result as map with fuel *)
+    have all_some: "\<forall>x \<in> set (map (\<lambda>(name, ty). case resolve_typedefs fuel typedefs ty of
+                                     None \<Rightarrow> None
+                                   | Some rty \<Rightarrow> Some (name, rty)) flds). x \<noteq> None"
+      using those_result those_Some_implies_all_Some
+      by metis
+
+    have map_eq: "\<forall>x \<in> set flds.
+          (case x of (name, ty) \<Rightarrow>
+            (case resolve_typedefs fuel'_pred typedefs ty of None \<Rightarrow> None | Some rty \<Rightarrow> Some (name, rty))) =
+          (case x of (name, ty) \<Rightarrow>
+            (case resolve_typedefs fuel typedefs ty of None \<Rightarrow> None | Some rty \<Rightarrow> Some (name, rty)))"
+    proof
+      fix x
+      assume x_in: "x \<in> set flds"
+      obtain name ty where x_def: "x = (name, ty)" by (cases x)
+      with x_in have name_ty_in: "(name, ty) \<in> set flds" by simp
+
+      (* The mapped element must be Some because those succeeded *)
+      have elem_form: "(case resolve_typedefs fuel typedefs ty of None \<Rightarrow> None | Some rty \<Rightarrow> Some (name, rty))
+                 \<in> set (map (\<lambda>(name, ty). case resolve_typedefs fuel typedefs ty of
+                                     None \<Rightarrow> None
+                                   | Some rty \<Rightarrow> Some (name, rty)) flds)"
+        using name_ty_in by auto
+      with all_some have not_none: "(case resolve_typedefs fuel typedefs ty of None \<Rightarrow> None | Some rty \<Rightarrow> Some (name, rty)) \<noteq> None"
+        by auto
+      then obtain rty where res_fuel: "resolve_typedefs fuel typedefs ty = Some rty"
+        by (auto split: option.splits)
+      with name_ty_in ih_all have res_fuel': "resolve_typedefs fuel'_pred typedefs ty = Some rty"
+        by blast
+      with res_fuel x_def show
+        "(case x of (name, ty) \<Rightarrow>
+            (case resolve_typedefs fuel'_pred typedefs ty of None \<Rightarrow> None | Some rty \<Rightarrow> Some (name, rty))) =
+         (case x of (name, ty) \<Rightarrow>
+            (case resolve_typedefs fuel typedefs ty of None \<Rightarrow> None | Some rty \<Rightarrow> Some (name, rty)))"
+        by simp
+    qed
+
+    have "those (map (\<lambda>(name, ty). case resolve_typedefs fuel'_pred typedefs ty of
+                                     None \<Rightarrow> None
+                                   | Some rty \<Rightarrow> Some (name, rty)) flds) =
+          those (map (\<lambda>(name, ty). case resolve_typedefs fuel typedefs ty of
+                                     None \<Rightarrow> None
+                                   | Some rty \<Rightarrow> Some (name, rty)) flds)"
+      using map_eq map_ext
+      by (metis (no_types, lifting)) 
+    with those_result have "those (map (\<lambda>(name, ty). case resolve_typedefs fuel'_pred typedefs ty of
+                                     None \<Rightarrow> None
+                                   | Some rty \<Rightarrow> Some (name, rty)) flds) = Some resolved_flds"
+      by simp
+
+    with Suc ty'_eq show ?thesis by simp
+  qed
+next
+  case (5 fuel typedefs loc ty dims)
+  (* BabTy_Array case *)
+  show ?case
+  proof (cases fuel')
+    case 0
+    with 5 show ?thesis by simp
+  next
+    case (Suc fuel'_pred)
+    with 5 have fuel_le: "fuel \<le> fuel'_pred"
+      by blast
+
+    (* The assumption tells us resolve_typedefs (Suc fuel) succeeded *)
+    (* which means resolve_typedefs fuel ty succeeded *)
+    from 5 have "resolve_typedefs (Suc fuel) typedefs (BabTy_Array loc ty dims) = Some ty'"
+      by blast
+    then obtain resolved_ty where
+      resolve_result: "resolve_typedefs fuel typedefs ty = Some resolved_ty"
+      and ty'_eq: "ty' = BabTy_Array loc resolved_ty dims"
+      by (auto split: option.splits)
+
+    (* Use IH for the element type *)
+    from resolve_result fuel_le "5.IH" have
+      "resolve_typedefs fuel'_pred typedefs ty = Some resolved_ty"
+      by blast
+
+    with Suc ty'_eq show ?thesis by simp
+  qed
+next
+  (* BabTy_Bool case *)
+  case ("6_1" fuel typedefs loc)
+  then show ?case by (cases fuel'; auto)
+next
+  (* BabTy_FiniteInt case *)
+  case ("6_2" fuel typedefs loc sign bits)
+  then show ?case by (cases fuel'; auto)
+next
+  (* BabTy_MathInt case *)
+  case ("6_3" fuel typedefs loc)
+  then show ?case by (cases fuel'; auto)
+next
+  (* BabTy_MathReal case *)
+  case ("6_4" fuel typedefs loc)
+  then show ?case by (cases fuel'; auto)
+qed
+
+
+(* resolve_typedefs is idempotent: resolving an already-resolved type gives the same result *)
+lemma resolve_typedefs_idempotent:
+  assumes "resolve_typedefs fuel typedefs ty = Some ty'"
+  shows "resolve_typedefs fuel typedefs ty' = Some ty'"
+  using assms
+proof (induction fuel typedefs ty arbitrary: ty' rule: resolve_typedefs.induct)
+  case (1 typedefs ty)
+  then show ?case by simp
+next
+  case (2 fuel typedefs loc name tyargs)
+  (* BabTy_Name case *)
+  from 2 obtain resolved_tyargs where
+    those_result: "those (map (resolve_typedefs fuel typedefs) tyargs) = Some resolved_tyargs"
+    by (auto split: option.splits)
+  show ?case
+  proof (cases "fmlookup typedefs name")
+    case None
+    (* Name not in typedefs - result is BabTy_Name with resolved tyargs *)
+    with 2 those_result have ty'_eq: "ty' = BabTy_Name loc name resolved_tyargs"
+      by auto
+    (* Each resolved_tyarg is idempotent by IH *)
+    have ih_tyargs: "\<forall>t \<in> set tyargs. \<forall>t'. resolve_typedefs fuel typedefs t = Some t' \<longrightarrow>
+                     resolve_typedefs fuel typedefs t' = Some t'"
+      using "2.IH" None by blast
+    (* Show that resolving resolved_tyargs gives resolved_tyargs *)
+    have all_some: "\<forall>t \<in> set (map (resolve_typedefs fuel typedefs) tyargs). t \<noteq> None"
+      using those_result those_Some_implies_all_Some by metis
+    have resolved_idempotent: "those (map (resolve_typedefs fuel typedefs) resolved_tyargs) = Some resolved_tyargs"
+    proof -
+      have "length resolved_tyargs = length tyargs"
+        using those_result by (metis length_map those_length)
+      moreover have "\<forall>i < length tyargs. resolve_typedefs fuel typedefs (resolved_tyargs ! i) = Some (resolved_tyargs ! i)"
+      proof (intro allI impI)
+        fix i assume i_bound: "i < length tyargs"
+        then have "tyargs ! i \<in> set tyargs" by simp
+        from those_nth[OF those_result] i_bound have
+          map_nth: "(map (resolve_typedefs fuel typedefs) tyargs) ! i = Some (resolved_tyargs ! i)"
+          by (simp add: \<open>length resolved_tyargs = length tyargs\<close>)
+        then have res: "resolve_typedefs fuel typedefs (tyargs ! i) = Some (resolved_tyargs ! i)"
+          using i_bound by simp
+        with ih_tyargs \<open>tyargs ! i \<in> set tyargs\<close> show "resolve_typedefs fuel typedefs (resolved_tyargs ! i) = Some (resolved_tyargs ! i)"
+          by auto
+      qed
+      ultimately show ?thesis
+        by (metis map_nth_eq_conv those_iff_all_Some)
+    qed
+    with ty'_eq None show ?thesis by simp
+  next
+    case (Some tydef)
+    then show ?thesis
+    proof (cases "DT_Definition tydef")
+      case None
+      (* Abstract type - result is BabTy_Name with resolved tyargs *)
+      with Some 2 those_result have ty'_eq: "ty' = BabTy_Name loc name resolved_tyargs"
+        by auto
+      have ih_tyargs: "\<forall>t \<in> set tyargs. \<forall>t'. resolve_typedefs fuel typedefs t = Some t' \<longrightarrow>
+                       resolve_typedefs fuel typedefs t' = Some t'"
+        using "2.IH" Some None by blast
+      have all_some: "\<forall>t \<in> set (map (resolve_typedefs fuel typedefs) tyargs). t \<noteq> None"
+        using those_result those_Some_implies_all_Some by metis
+      have resolved_idempotent: "those (map (resolve_typedefs fuel typedefs) resolved_tyargs) = Some resolved_tyargs"
+      proof -
+        have "length resolved_tyargs = length tyargs"
+          using those_result by (metis length_map those_length)
+        moreover have "\<forall>i < length tyargs. resolve_typedefs fuel typedefs (resolved_tyargs ! i) = Some (resolved_tyargs ! i)"
+        proof (intro allI impI)
+          fix i assume i_bound: "i < length tyargs"
+          then have "tyargs ! i \<in> set tyargs" by simp
+          from those_nth[OF those_result] i_bound have
+            map_nth: "(map (resolve_typedefs fuel typedefs) tyargs) ! i = Some (resolved_tyargs ! i)"
+            by (simp add: \<open>length resolved_tyargs = length tyargs\<close>)
+          then have res: "resolve_typedefs fuel typedefs (tyargs ! i) = Some (resolved_tyargs ! i)"
+            using i_bound by simp
+          with ih_tyargs \<open>tyargs ! i \<in> set tyargs\<close> show "resolve_typedefs fuel typedefs (resolved_tyargs ! i) = Some (resolved_tyargs ! i)"
+            by auto
+        qed
+        ultimately show ?thesis
+          by (metis map_nth_eq_conv those_iff_all_Some)
+      qed
+      with ty'_eq Some None show ?thesis by simp
+    next
+      case (Some body)
+      (* Concrete typedef - recursively resolved *)
+      define typarams where "typarams = DT_TyArgs tydef"
+      define subst where "subst = fmap_of_list (zip typarams resolved_tyargs)"
+      define subst_body where "subst_body = substitute_bab_type subst body"
+      from \<open>fmlookup typedefs name = Some tydef\<close> Some those_result 2 have
+        res_subst: "resolve_typedefs fuel typedefs subst_body = Some ty'"
+        by (simp add: typarams_def subst_def subst_body_def)
+      (* Use the IH for the substituted body *)
+      from "2.IH"(2)
+      have "resolve_typedefs fuel typedefs ty' = Some ty'"
+        using Some \<open>fmlookup typedefs name = Some tydef\<close> res_subst subst_body_def subst_def
+          those_result typarams_def by blast
+      then show ?thesis
+        using resolve_typedefs_monotonic[of fuel typedefs ty' ty' "Suc fuel"] by simp
+    qed
+  qed
+next
+  case (3 fuel typedefs loc tys)
+  (* BabTy_Tuple case *)
+  from 3 obtain resolved_tys where
+    those_result: "those (map (resolve_typedefs fuel typedefs) tys) = Some resolved_tys"
+    and ty'_eq: "ty' = BabTy_Tuple loc resolved_tys"
+    by (auto split: option.splits)
+  have ih_tys: "\<forall>t \<in> set tys. \<forall>t'. resolve_typedefs fuel typedefs t = Some t' \<longrightarrow>
+               resolve_typedefs fuel typedefs t' = Some t'"
+    using "3.IH" by blast
+  have all_some: "\<forall>t \<in> set (map (resolve_typedefs fuel typedefs) tys). t \<noteq> None"
+    using those_result those_Some_implies_all_Some by metis
+  have resolved_idempotent: "those (map (resolve_typedefs fuel typedefs) resolved_tys) = Some resolved_tys"
+  proof -
+    have "length resolved_tys = length tys"
+      using those_result by (metis length_map those_length)
+    moreover have "\<forall>i < length tys. resolve_typedefs fuel typedefs (resolved_tys ! i) = Some (resolved_tys ! i)"
+    proof (intro allI impI)
+      fix i assume i_bound: "i < length tys"
+      then have "tys ! i \<in> set tys" by simp
+      from those_nth[OF those_result] i_bound have
+        map_nth: "(map (resolve_typedefs fuel typedefs) tys) ! i = Some (resolved_tys ! i)"
+        by (simp add: \<open>length resolved_tys = length tys\<close>)
+      then have res: "resolve_typedefs fuel typedefs (tys ! i) = Some (resolved_tys ! i)"
+        using i_bound by simp
+      with ih_tys \<open>tys ! i \<in> set tys\<close> show "resolve_typedefs fuel typedefs (resolved_tys ! i) = Some (resolved_tys ! i)"
+        by auto
+    qed
+    ultimately show ?thesis
+      by (metis map_nth_eq_conv those_iff_all_Some)
+  qed
+  with ty'_eq show ?case by simp
+next
+  case (4 fuel typedefs loc flds)
+  (* BabTy_Record case *)
+  let ?map_fld = "\<lambda>(name, ty). case resolve_typedefs fuel typedefs ty of None \<Rightarrow> None | Some rty \<Rightarrow> Some (name, rty)"
+  from 4 obtain resolved_flds where
+    those_result: "those (map ?map_fld flds) = Some resolved_flds"
+    and ty'_eq: "ty' = BabTy_Record loc resolved_flds"
+    by (auto split: option.splits)
+  have ih_flds: "\<forall>(name, ty) \<in> set flds. \<forall>ty'. resolve_typedefs fuel typedefs ty = Some ty' \<longrightarrow>
+               resolve_typedefs fuel typedefs ty' = Some ty'"
+    using "4.IH" by blast
+  have all_some: "\<forall>x \<in> set (map ?map_fld flds). x \<noteq> None"
+    using those_result those_Some_implies_all_Some by metis
+  (* Show that resolved_flds has same length as flds and each field type is idempotent *)
+  have len_eq: "length resolved_flds = length flds"
+    using those_result by (metis length_map those_length)
+  have resolved_idempotent: "those (map ?map_fld resolved_flds) = Some resolved_flds"
+  proof -
+    have "\<forall>i < length flds. ?map_fld (resolved_flds ! i) = Some (resolved_flds ! i)"
+    proof (intro allI impI)
+      fix i assume i_bound: "i < length flds"
+      (* Get the i-th field from flds *)
+      obtain fname fty where fld_i: "flds ! i = (fname, fty)" by (cases "flds ! i")
+      then have "(fname, fty) \<in> set flds" using i_bound
+        by (metis nth_mem) 
+      (* From those_result, the i-th mapped element is Some (resolved_flds ! i) *)
+      from those_nth[OF those_result] i_bound have
+        map_nth: "(map ?map_fld flds) ! i = Some (resolved_flds ! i)"
+        by (simp add: len_eq)
+      then have "?map_fld (flds ! i) = Some (resolved_flds ! i)"
+        using i_bound by simp
+      with fld_i obtain rty where
+        res_fty: "resolve_typedefs fuel typedefs fty = Some rty"
+        and resolved_i: "resolved_flds ! i = (fname, rty)"
+        by (auto split: option.splits)
+      (* By IH, resolving rty again gives rty *)
+      from ih_flds \<open>(fname, fty) \<in> set flds\<close> res_fty have
+        "resolve_typedefs fuel typedefs rty = Some rty" by auto
+      with resolved_i show "?map_fld (resolved_flds ! i) = Some (resolved_flds ! i)"
+        by simp
+    qed
+    with len_eq show ?thesis
+      by (simp add: those_iff_all_Some)
+  qed
+  with ty'_eq show ?case by simp
+next
+  case (5 fuel typedefs loc ty dims)
+  (* BabTy_Array case *)
+  from 5 obtain resolved_ty where
+    resolve_result: "resolve_typedefs fuel typedefs ty = Some resolved_ty"
+    and ty'_eq: "ty' = BabTy_Array loc resolved_ty dims"
+    by (auto split: option.splits)
+  from "5.IH"[OF resolve_result] have ih: "resolve_typedefs fuel typedefs resolved_ty = Some resolved_ty"
+    by simp
+  with ty'_eq show ?case by simp
+next
+  (* Base types - BabTy_Bool *)
+  case ("6_1" fuel typedefs loc)
+  then show ?case by auto
+next
+  (* Base types - BabTy_FiniteInt *)
+  case ("6_2" fuel typedefs loc sign bits)
+  then show ?case by auto
+next
+  (* Base types - BabTy_MathInt *)
+  case ("6_3" fuel typedefs loc)
+  then show ?case by auto
+next
+  (* Base types - BabTy_MathReal *)
+  case ("6_4" fuel typedefs loc)
+  then show ?case by auto
+qed
+
+end
