isabelle/TypeEnv.thy
@@ -1,0 +1,608 @@
+theory TypeEnv
+  imports BabSyntax
+begin
+
+record BabTyEnv =
+  (* Term-level bindings: variables and constants *)
+  (* Types are kind-correct and all typedefs are resolved *)
+  TE_TermVars :: "(string, BabType) fmap"
+
+  (* Ghost variables - subset of TE_TermVars keys *)
+  TE_GhostVars :: "string fset"
+
+  (* Type variable bindings: for polymorphic contexts *)
+  TE_TypeVars :: "string fset"
+
+  (* Function signatures *)
+  (* DeclFuns are valid and have all typedefs resolved *)
+  TE_Functions :: "(string, DeclFun) fmap"
+
+  (* Datatype definitions *)
+  (* DeclDatatypes are valid and have all typedefs resolved *)
+  TE_Datatypes :: "(string, DeclDatatype) fmap"
+
+
+(* Helper functions for BabTyEnv *)
+
+(* Add a variable to the environment *)
+(*
+fun add_var :: "string \<Rightarrow> BabType \<Rightarrow> GhostOrNot \<Rightarrow> BabTyEnv \<Rightarrow> BabTyEnv" where
+  "add_var name ty Ghost env =
+    env \<lparr> TE_TermVars := fmupd name ty (TE_TermVars env),
+          TE_GhostVars := finsert name (TE_GhostVars env) \<rparr>"
+| "add_var name ty NotGhost env =
+    env \<lparr> TE_TermVars := fmupd name ty (TE_TermVars env) \<rparr>"
+*)
+
+(* Add a type variable to the environment *)
+(*
+fun add_type_var :: "string \<Rightarrow> BabTyEnv \<Rightarrow> BabTyEnv" where
+  "add_type_var name env = env \<lparr> TE_TypeVars := finsert name (TE_TypeVars env) \<rparr>"
+*)
+
+(* Clear local variables (for entering a new function scope) *)
+(*
+fun clear_locals :: "BabTyEnv \<Rightarrow> BabTyEnv" where
+  "clear_locals env = env \<lparr> TE_TermVars := fmempty, TE_GhostVars := {||}, TE_TypeVars := {||} \<rparr>"
+*)
+
+(* Check if a type is an integer type *)
+fun is_integer_type :: "BabType \<Rightarrow> bool" where
+  "is_integer_type (BabTy_FiniteInt _ _ _) = True"
+| "is_integer_type (BabTy_MathInt _) = True"
+| "is_integer_type _ = False"
+
+(* Check if a type is a signed integer type (signed finite int or MathInt) *)
+fun is_signed_integer_type :: "BabType \<Rightarrow> bool" where
+  "is_signed_integer_type (BabTy_FiniteInt _ Signed _) = True"
+| "is_signed_integer_type (BabTy_MathInt _) = True"
+| "is_signed_integer_type _ = False"
+
+(* Check if a type is a finite integer type *)
+fun is_finite_integer_type :: "BabType \<Rightarrow> bool" where
+  "is_finite_integer_type (BabTy_FiniteInt _ _ _) = True"
+| "is_finite_integer_type _ = False"
+
+(* Check if an array dimension is resolved (not BabDim_Fixed) *)
+fun is_resolved_dimension :: "BabDimension \<Rightarrow> bool" where
+  "is_resolved_dimension (BabDim_Fixed _) = False"
+| "is_resolved_dimension _ = True"
+
+(* Check if a type is a runtime-compatible type (no MathInt/MathReal) *)
+fun is_runtime_type :: "BabType \<Rightarrow> bool" where
+  "is_runtime_type (BabTy_MathInt _) = False"
+| "is_runtime_type (BabTy_MathReal _) = False"
+| "is_runtime_type (BabTy_Tuple _ tys) = list_all is_runtime_type tys"
+| "is_runtime_type (BabTy_Record _ flds) = list_all (is_runtime_type \<circ> snd) flds"
+| "is_runtime_type (BabTy_Array _ ty _) = is_runtime_type ty"
+| "is_runtime_type _ = True"
+
+
+(* Check structural equality of types *)
+(* This only works on fully resolved types, i.e. typedefs are not followed *)
+function types_equal :: "BabType \<Rightarrow> BabType \<Rightarrow> bool" where
+  "types_equal ty1 ty2 =
+    (case (ty1, ty2) of
+      (BabTy_Bool _, BabTy_Bool _) \<Rightarrow> True
+    | (BabTy_FiniteInt _ s1 b1, BabTy_FiniteInt _ s2 b2) \<Rightarrow> (s1 = s2 \<and> b1 = b2)
+    | (BabTy_MathInt _, BabTy_MathInt _) \<Rightarrow> True
+    | (BabTy_MathReal _, BabTy_MathReal _) \<Rightarrow> True
+    | (BabTy_Tuple _ tys1, BabTy_Tuple _ tys2) \<Rightarrow>
+        (length tys1 = length tys2 \<and>
+         list_all (\<lambda>(t1, t2). types_equal t1 t2) (zip tys1 tys2))
+    | (BabTy_Record _ flds1, BabTy_Record _ flds2) \<Rightarrow>
+        (length flds1 = length flds2 \<and>
+         list_all (\<lambda>(fld1, fld2). fst fld1 = fst fld2 \<and> types_equal (snd fld1) (snd fld2))
+                 (zip flds1 flds2))
+    | (BabTy_Array _ elem1 dims1, BabTy_Array _ elem2 dims2) \<Rightarrow>
+        (dims1 = dims2 \<and> types_equal elem1 elem2)
+    | (BabTy_Name _ n1 tyargs1, BabTy_Name _ n2 tyargs2) \<Rightarrow>
+        (n1 = n2 \<and> 
+         length tyargs1 = length tyargs2 \<and>
+         list_all (\<lambda>(ta1, ta2). types_equal ta1 ta2) (zip tyargs1 tyargs2))
+    | _ \<Rightarrow> False)"
+  by pat_completeness auto
+
+termination types_equal
+proof (relation "measure (\<lambda>(t1, t2). bab_type_size t1 + bab_type_size t2)")
+  show "wf (measure (\<lambda>(t1, t2). bab_type_size t1 + bab_type_size t2))"
+    by auto
+next
+  (* BabTy_Name case: type arguments in zip are smaller *)
+  fix ty1 ty2 x y x11 x12 x13 x11a x12a x13a z xa ya
+  assume xy: "(x, y) = (ty1, ty2)"
+     and x: "x = BabTy_Name x11 x12 x13"
+     and y: "y = BabTy_Name x11a x12a x13a"
+     and z: "z \<in> set (zip x13 x13a)"
+     and xaya: "(xa, ya) = z"
+  have "bab_type_size xa < Suc (sum_list (map bab_type_size x13))"
+    by (metis bab_type_smaller_than_list in_set_zipE xaya z)
+  hence "bab_type_size xa < bab_type_size ty1"
+    using x xy by fastforce
+  moreover have "bab_type_size ya < Suc (sum_list (map bab_type_size x13a))"
+    by (metis bab_type_smaller_than_list set_zip_rightD xaya z)
+  hence "bab_type_size ya < bab_type_size ty2"
+    by (metis bab_type_size.simps(1) plus_1_eq_Suc prod.inject xy y)
+  ultimately show "((xa, ya), ty1, ty2) \<in> measure (\<lambda>(t1, t2). bab_type_size t1 + bab_type_size t2)"
+    by simp
+next
+  (* Tuple case: elements in zip are smaller *)
+  fix ty1 ty2 x y x61 x62 x61a x62a z xa ya
+  assume xy: "(x, y) = (ty1, ty2)"
+     and x: "x = BabTy_Tuple x61 x62"
+     and y: "y = BabTy_Tuple x61a x62a"
+     and z: "z \<in> set (zip x62 x62a)"
+     and xaya: "(xa, ya) = z"
+  have "bab_type_size xa < Suc (sum_list (map bab_type_size x62))"
+    by (metis bab_type_smaller_than_list in_set_zipE xaya z)
+  hence "bab_type_size xa < bab_type_size ty1"
+    using x xy by fastforce
+  moreover have "bab_type_size ya < Suc (sum_list (map bab_type_size x62a))"
+    by (metis bab_type_smaller_than_list set_zip_rightD xaya z)
+  hence "bab_type_size ya < bab_type_size ty2"
+    by (metis bab_type_size.simps(6) plus_1_eq_Suc prod.inject xy y)
+  ultimately show "((xa, ya), ty1, ty2) \<in> measure (\<lambda>(t1, t2). bab_type_size t1 + bab_type_size t2)"
+    by simp
+next
+  (* Record case: field types in zip are smaller *)
+  fix ty1 ty2 x y x71 x72 x71a x72a z fld1 fld2
+  assume xy: "(x, y) = (ty1, ty2)"
+     and x: "x = BabTy_Record x71 x72"
+     and y: "y = BabTy_Record x71a x72a"
+     and z: "z \<in> set (zip x72 x72a)"
+     and fld12: "(fld1, fld2) = z"
+  have "fld1 \<in> set x72"
+    by (metis fld12 in_set_zipE z)
+  hence "snd fld1 \<in> snd ` set x72"
+    by force
+  hence "bab_type_size (snd fld1) < Suc (sum_list (map (bab_type_size \<circ> snd) x72))"
+    using bab_type_smaller_than_fieldlist by fastforce
+  hence "bab_type_size (snd fld1) < bab_type_size ty1"
+    using x xy by fastforce
+  moreover have "fld2 \<in> set x72a"
+    by (metis fld12 set_zip_rightD z)
+  hence "snd fld2 \<in> snd ` set x72a"
+    by force
+  hence "bab_type_size (snd fld2) < Suc (sum_list (map (bab_type_size \<circ> snd) x72a))"
+    using bab_type_smaller_than_fieldlist by fastforce
+  hence "bab_type_size (snd fld2) < bab_type_size ty2"
+    by (metis bab_type_size.simps(7) plus_1_eq_Suc prod.inject xy y)
+  ultimately show "((snd fld1, snd fld2), ty1, ty2) \<in> measure (\<lambda>(t1, t2). bab_type_size t1 + bab_type_size t2)"
+    by simp
+next
+  (* Array case: element types are smaller *)
+  fix ty1 ty2 x y x81 x82 x83 x81a x82a x83a
+  assume xy: "(x, y) = (ty1, ty2)"
+     and x: "x = BabTy_Array x81 x82 x83"
+     and y: "y = BabTy_Array x81a x82a x83a"
+  have "bab_type_size x82 < bab_type_size ty1"
+    using x xy by fastforce
+  moreover have "bab_type_size x82a < bab_type_size ty2"
+    using y xy by fastforce
+  ultimately show "((x82, x82a), ty1, ty2) \<in> measure (\<lambda>(ty1, ty2). bab_type_size ty1 + bab_type_size ty2)"
+    by simp
+qed
+
+
+(* Simplification lemmas for types_equal *)
+lemma types_equal_Tuple:
+  "types_equal (BabTy_Tuple loc1 tys1) (BabTy_Tuple loc2 tys2) =
+   (length tys1 = length tys2 \<and> list_all (\<lambda>(t1, t2). types_equal t1 t2) (zip tys1 tys2))"
+  by (smt (verit, best) BabType.simps(70) old.prod.case types_equal.simps)
+
+lemma types_equal_Name:
+  "types_equal (BabTy_Name loc1 n1 tyargs1) (BabTy_Name loc2 n2 tyargs2) =
+   (n1 = n2 \<and> length tyargs1 = length tyargs2 \<and>
+    list_all (\<lambda>(ta1, ta2). types_equal ta1 ta2) (zip tyargs1 tyargs2))"
+  by (smt (verit) BabType.simps(65) old.prod.case types_equal.simps)
+
+
+(* Proving that types_equal is an equivalence relation: *)
+
+(* Helper: zip of a list with itself gives paired elements *)
+lemma zip_same_list_all:
+  "list_all (\<lambda>(x, y). P x y) (zip xs xs) \<longleftrightarrow> list_all (\<lambda>x. P x x) xs"
+  by (induction xs) auto
+
+(* types_equal is reflexive *)
+lemma types_equal_reflexive:
+  "types_equal ty ty"
+proof (induction ty rule: measure_induct_rule[where f=bab_type_size])
+  case (less ty)
+  then show ?case
+  proof (cases ty)
+    case (BabTy_Bool loc)
+    then show ?thesis by simp
+  next
+    case (BabTy_FiniteInt loc s b)
+    then show ?thesis by simp
+  next
+    case (BabTy_MathInt loc)
+    then show ?thesis by simp
+  next
+    case (BabTy_MathReal loc)
+    then show ?thesis by simp
+  next
+    case (BabTy_Tuple loc tys)
+    have "\<And>t. t \<in> set tys \<Longrightarrow> types_equal t t"
+      using less BabTy_Tuple bab_type_smaller_than_list by fastforce
+    then have "list_all (\<lambda>t. types_equal t t) tys"
+      by (simp add: list_all_iff)
+    then show ?thesis
+      using BabTy_Tuple zip_same_list_all types_equal_Tuple by fastforce
+  next
+    case (BabTy_Record loc flds)
+    have "\<And>fld. fld \<in> set flds \<Longrightarrow> types_equal (snd fld) (snd fld)"
+      using less BabTy_Record bab_type_smaller_than_fieldlist by fastforce
+    then have "list_all (\<lambda>fld. types_equal (snd fld) (snd fld)) flds"
+      by (simp add: list_all_iff)
+    then have "list_all (\<lambda>(fld1, fld2). fst fld1 = fst fld2 \<and> types_equal (snd fld1) (snd fld2)) (zip flds flds)"
+      by (simp add: zip_same_list_all)
+    then show ?thesis
+      using BabTy_Record by simp
+  next
+    case (BabTy_Array loc elem dims)
+    then show ?thesis using less by simp
+  next
+    case (BabTy_Name loc n tyargs)
+    have "\<And>t. t \<in> set tyargs \<Longrightarrow> types_equal t t"
+      using less BabTy_Name bab_type_smaller_than_list by fastforce
+    then have "list_all (\<lambda>t. types_equal t t) tyargs"
+      by (simp add: list_all_iff)
+    then show ?thesis
+      using BabTy_Name zip_same_list_all types_equal_Name by fastforce
+  qed
+qed
+
+(* Helper: if a symmetric property holds for all pairs in two equal-length lists,
+   then list_all holds symmetrically *)
+lemma list_all_zip_symmetric:
+  assumes "\<forall>x y. (x, y) \<in> set (zip xs ys) \<longrightarrow> P x y = P y x"
+    and "length xs = length ys"
+  shows "list_all (\<lambda>(x, y). P x y) (zip xs ys) = list_all (\<lambda>(x, y). P x y) (zip ys xs)"
+  using assms
+  by (auto simp: list_all_length set_zip)
+
+(* types_equal is symmetric *)
+lemma types_equal_symmetric:
+  "types_equal ty1 ty2 = types_equal ty2 ty1"
+proof (induction ty1 ty2 rule: types_equal.induct)
+  case (1 ty1 ty2)
+  show ?case
+  proof (cases ty1)
+    case (BabTy_Bool loc1)
+    then show ?thesis by (cases ty2; simp)
+  next
+    case (BabTy_FiniteInt loc1 s1 b1)
+    then show ?thesis by (cases ty2; auto)
+  next
+    case (BabTy_MathInt loc1)
+    then show ?thesis by (cases ty2; simp)
+  next
+    case (BabTy_MathReal loc1)
+    then show ?thesis by (cases ty2; simp)
+  next
+    case tuple1: (BabTy_Tuple loc1 tys1)
+    then show ?thesis
+    proof (cases ty2)
+      case tuple2: (BabTy_Tuple loc2 tys2)
+      show ?thesis
+        using tuple1 tuple2 types_equal_Tuple list_all_zip_symmetric
+        by (metis (mono_tags, lifting) "1.IH"(2)) 
+    qed auto
+  next
+    case record1: (BabTy_Record loc1 flds1)
+    then show ?thesis
+    proof (cases ty2)
+      case record2: (BabTy_Record loc2 flds2)
+      show ?thesis
+        using record1 record2 list_all_zip_symmetric
+        by (smt (verit, best) "1.IH"(3) BabType.simps(71) case_prodD case_prodI
+            types_equal.simps)
+    qed auto
+  next
+    case array1: (BabTy_Array loc1 elem1 dims1)
+    then show ?thesis
+    proof (cases ty2)
+      case array2: (BabTy_Array loc2 elem2 dims2)
+      show ?thesis
+        using array1 array2 "1.IH"(4) by auto
+    qed auto
+  next
+    case name1: (BabTy_Name loc1 n1 tyargs1)
+    then show ?thesis
+    proof (cases ty2)
+      case name2: (BabTy_Name loc2 n2 tyargs2)
+      show ?thesis
+        using name1 name2 types_equal_Name list_all_zip_symmetric
+        by (metis (full_types) "1.IH"(1))
+    qed auto
+  qed
+qed
+
+(* Helper for transitivity: zip three lists *)
+lemma list_all_zip3_trans:
+  assumes "length xs = length ys" "length ys = length zs"
+    and "list_all (\<lambda>(x, y). P x y) (zip xs ys)"
+    and "list_all (\<lambda>(y, z). P y z) (zip ys zs)"
+    and "\<And>x y z. (x, y) \<in> set (zip xs ys) \<Longrightarrow> P x y \<Longrightarrow> P y z \<Longrightarrow> P x z"
+  shows "list_all (\<lambda>(x, z). P x z) (zip xs zs)"
+  using assms
+  by (induction xs ys zs rule: list_induct3) auto
+
+(* types_equal is transitive *)
+lemma types_equal_transitive:
+  "types_equal ty1 ty2 \<Longrightarrow> types_equal ty2 ty3 \<Longrightarrow> types_equal ty1 ty3"
+proof (induction ty1 ty2 arbitrary: ty3 rule: types_equal.induct)
+  case (1 ty1 ty2)
+  show ?case
+  proof (cases ty1)
+    case (BabTy_Bool loc1)
+    then show ?thesis using "1.prems" by (cases ty2; cases ty3; simp)
+  next
+    case (BabTy_FiniteInt loc1 s1 b1)
+    then show ?thesis using "1.prems" by (cases ty2; cases ty3; auto)
+  next
+    case (BabTy_MathInt loc1)
+    then show ?thesis using "1.prems" by (cases ty2; cases ty3; simp)
+  next
+    case (BabTy_MathReal loc1)
+    then show ?thesis using "1.prems" by (cases ty2; cases ty3; simp)
+  next
+    case tuple1: (BabTy_Tuple loc1 tys1)
+    then show ?thesis using "1.prems"
+    proof (cases ty2)
+      case tuple2: (BabTy_Tuple loc2 tys2)
+      then show ?thesis using "1.prems" tuple1
+      proof (cases ty3)
+        case tuple3: (BabTy_Tuple loc3 tys3)
+        from "1.prems" tuple1 tuple2 have eq12: "types_equal ty1 ty2" by simp
+        from "1.prems" tuple2 tuple3 have eq23: "types_equal ty2 ty3" by simp
+        from eq12 tuple1 tuple2 have len12: "length tys1 = length tys2"
+          and all12: "list_all (\<lambda>(t1, t2). types_equal t1 t2) (zip tys1 tys2)"
+          using types_equal_Tuple by auto
+        from eq23 tuple2 tuple3 have len23: "length tys2 = length tys3"
+          and all23: "list_all (\<lambda>(t2, t3). types_equal t2 t3) (zip tys2 tys3)"
+          using types_equal_Tuple by auto
+        have "list_all (\<lambda>(t1, t3). types_equal t1 t3) (zip tys1 tys3)"
+          using list_all_zip3_trans[OF len12 len23 all12 all23] "1.IH"(2) tuple1 tuple2
+          by fastforce
+        then show ?thesis
+          using tuple1 tuple3 len12 len23 types_equal_Tuple by auto
+      next
+        case (BabTy_Name x11 x12 x13)
+        then show ?thesis using "1.prems" tuple2 by simp
+      next
+        case (BabTy_Bool x2)
+        then show ?thesis using "1.prems" tuple2 by simp
+      next
+        case (BabTy_FiniteInt x31 x32 x33)
+        then show ?thesis using "1.prems" tuple2 by simp
+      next
+        case (BabTy_MathInt x4)
+        then show ?thesis using "1.prems" tuple2 by simp
+      next
+        case (BabTy_MathReal x5)
+        then show ?thesis using "1.prems" tuple2 by simp
+      next
+        case (BabTy_Record x71 x72)
+        then show ?thesis using "1.prems" tuple2 by simp
+      next
+        case (BabTy_Array x81 x82 x83)
+        then show ?thesis using "1.prems" tuple2 by simp
+      qed
+    next
+      case (BabTy_Name x11 x12 x13)
+      then show ?thesis using "1.prems" tuple1 by simp
+    next
+      case (BabTy_Bool x2)
+      then show ?thesis using "1.prems" tuple1 by simp
+    next
+      case (BabTy_FiniteInt x31 x32 x33)
+      then show ?thesis using "1.prems" tuple1 by simp
+    next
+      case (BabTy_MathInt x4)
+      then show ?thesis using "1.prems" tuple1 by simp
+    next
+      case (BabTy_MathReal x5)
+      then show ?thesis using "1.prems" tuple1 by simp
+    next
+      case (BabTy_Record x71 x72)
+      then show ?thesis using "1.prems" tuple1 by simp
+    next
+      case (BabTy_Array x81 x82 x83)
+      then show ?thesis using "1.prems" tuple1 by simp
+    qed
+  next
+    case record1: (BabTy_Record loc1 flds1)
+    then show ?thesis using "1.prems"
+    proof (cases ty2)
+      case record2: (BabTy_Record loc2 flds2)
+      then show ?thesis using "1.prems" record1
+      proof (cases ty3)
+        case (BabTy_Record loc3 flds3)
+        from "1.prems" record1 record2 have eq12: "types_equal ty1 ty2" by simp
+        from "1.prems" record2 BabTy_Record have eq23: "types_equal ty2 ty3" by simp
+        from eq12 record1 record2 have len12: "length flds1 = length flds2"
+          and all12: "list_all (\<lambda>(f1, f2). fst f1 = fst f2 \<and> types_equal (snd f1) (snd f2)) (zip flds1 flds2)"
+          by auto
+        from eq23 record2 BabTy_Record have len23: "length flds2 = length flds3"
+          and all23: "list_all (\<lambda>(f2, f3). fst f2 = fst f3 \<and> types_equal (snd f2) (snd f3)) (zip flds2 flds3)"
+          by auto
+        have "list_all (\<lambda>(f1, f3). fst f1 = fst f3 \<and> types_equal (snd f1) (snd f3)) (zip flds1 flds3)"
+          using list_all_zip3_trans[OF len12 len23,
+                  of "\<lambda>f1 f2. fst f1 = fst f2 \<and> types_equal (snd f1) (snd f2)"]
+                all12 all23 "1.IH"(3) record1 record2
+          by presburger
+        then show ?thesis
+          using record1 BabTy_Record len12 len23 by auto
+      next
+        case (BabTy_Name x11 x12 x13)
+        then show ?thesis using "1.prems" record2 by simp
+      next
+        case (BabTy_Bool x2)
+        then show ?thesis using "1.prems" record2 by simp
+      next
+        case (BabTy_FiniteInt x31 x32 x33)
+        then show ?thesis using "1.prems" record2 by simp
+      next
+        case (BabTy_MathInt x4)
+        then show ?thesis using "1.prems" record2 by simp
+      next
+        case (BabTy_MathReal x5)
+        then show ?thesis using "1.prems" record2 by simp
+      next
+        case (BabTy_Tuple x61 x62)
+        then show ?thesis using "1.prems" record2 by simp
+      next
+        case (BabTy_Array x81 x82 x83)
+        then show ?thesis using "1.prems" record2 by simp
+      qed
+    next
+      case (BabTy_Name x11 x12 x13)
+      then show ?thesis using "1.prems" record1 by simp
+    next
+      case (BabTy_Bool x2)
+      then show ?thesis using "1.prems" record1 by simp
+    next
+      case (BabTy_FiniteInt x31 x32 x33)
+      then show ?thesis using "1.prems" record1 by simp
+    next
+      case (BabTy_MathInt x4)
+      then show ?thesis using "1.prems" record1 by simp
+    next
+      case (BabTy_MathReal x5)
+      then show ?thesis using "1.prems" record1 by simp
+    next
+      case (BabTy_Tuple x61 x62)
+      then show ?thesis using "1.prems" record1 by simp
+    next
+      case (BabTy_Array x81 x82 x83)
+      then show ?thesis using "1.prems" record1 by simp
+    qed
+  next
+    case array1: (BabTy_Array loc1 elem1 dims1)
+    then show ?thesis using "1.prems"
+    proof (cases ty2)
+      case array2: (BabTy_Array loc2 elem2 dims2)
+      then show ?thesis using "1.prems" array1
+      proof (cases ty3)
+        case array3: (BabTy_Array loc3 elem3 dims3)
+        then show ?thesis
+          using "1.prems" "1.IH"(4) array1 array2 by auto
+      next
+        case (BabTy_Name x11 x12 x13)
+        then show ?thesis using "1.prems" array2 by simp
+      next
+        case (BabTy_Bool x2)
+        then show ?thesis using "1.prems" array2 by simp
+      next
+        case (BabTy_FiniteInt x31 x32 x33)
+        then show ?thesis using "1.prems" array2 by simp
+      next
+        case (BabTy_MathInt x4)
+        then show ?thesis using "1.prems" array2 by simp
+      next
+        case (BabTy_MathReal x5)
+        then show ?thesis using "1.prems" array2 by simp
+      next
+        case (BabTy_Tuple x61 x62)
+        then show ?thesis using "1.prems" array2 by simp
+      next
+        case (BabTy_Record x71 x72)
+        then show ?thesis using "1.prems" array2 by simp
+      qed
+    next
+      case (BabTy_Name x11 x12 x13)
+      then show ?thesis using "1.prems" array1 by simp
+    next
+      case (BabTy_Bool x2)
+      then show ?thesis using "1.prems" array1 by simp
+    next
+      case (BabTy_FiniteInt x31 x32 x33)
+      then show ?thesis using "1.prems" array1 by simp
+    next
+      case (BabTy_MathInt x4)
+      then show ?thesis using "1.prems" array1 by simp
+    next
+      case (BabTy_MathReal x5)
+      then show ?thesis using "1.prems" array1 by simp
+    next
+      case (BabTy_Tuple x61 x62)
+      then show ?thesis using "1.prems" array1 by simp
+    next
+      case (BabTy_Record x71 x72)
+      then show ?thesis using "1.prems" array1 by simp
+    qed
+  next
+    case name1: (BabTy_Name loc1 n1 tyargs1)
+    then show ?thesis using "1.prems"
+    proof (cases ty2)
+      case name2: (BabTy_Name loc2 n2 tyargs2)
+      then show ?thesis using "1.prems" name1
+      proof (cases ty3)
+        case name3: (BabTy_Name loc3 n3 tyargs3)
+        from "1.prems" name1 name2 have eq12: "types_equal ty1 ty2" by simp
+        from "1.prems" name2 name3 have eq23: "types_equal ty2 ty3" by simp
+        from eq12 name1 name2 have n_eq1: "n1 = n2"
+          and len12: "length tyargs1 = length tyargs2"
+          and all12: "list_all (\<lambda>(t1, t2). types_equal t1 t2) (zip tyargs1 tyargs2)"
+          using types_equal_Name by auto
+        from eq23 name2 name3 have n_eq2: "n2 = n3"
+          and len23: "length tyargs2 = length tyargs3"
+          and all23: "list_all (\<lambda>(t2, t3). types_equal t2 t3) (zip tyargs2 tyargs3)"
+          using types_equal_Name by auto
+        have "list_all (\<lambda>(t1, t3). types_equal t1 t3) (zip tyargs1 tyargs3)"
+          using list_all_zip3_trans[OF len12 len23 all12 all23] "1.IH"(1) name1 name2
+          by fastforce
+        then show ?thesis
+          using name1 name3 n_eq1 n_eq2 len12 len23 types_equal_Name by auto
+      next
+        case (BabTy_Bool x2)
+        then show ?thesis using "1.prems" name2 by simp
+      next
+        case (BabTy_FiniteInt x31 x32 x33)
+        then show ?thesis using "1.prems" name2 by simp
+      next
+        case (BabTy_MathInt x4)
+        then show ?thesis using "1.prems" name2 by simp
+      next
+        case (BabTy_MathReal x5)
+        then show ?thesis using "1.prems" name2 by simp
+      next
+        case (BabTy_Tuple x61 x62)
+        then show ?thesis using "1.prems" name2 by simp
+      next
+        case (BabTy_Record x71 x72)
+        then show ?thesis using "1.prems" name2 by simp
+      next
+        case (BabTy_Array x81 x82 x83)
+        then show ?thesis using "1.prems" name2 by simp
+      qed
+    next
+      case (BabTy_Bool x2)
+      then show ?thesis using "1.prems" name1 by simp
+    next
+      case (BabTy_FiniteInt x31 x32 x33)
+      then show ?thesis using "1.prems" name1 by simp
+    next
+      case (BabTy_MathInt x4)
+      then show ?thesis using "1.prems" name1 by simp
+    next
+      case (BabTy_MathReal x5)
+      then show ?thesis using "1.prems" name1 by simp
+    next
+      case (BabTy_Tuple x61 x62)
+      then show ?thesis using "1.prems" name1 by simp
+    next
+      case (BabTy_Record x71 x72)
+      then show ?thesis using "1.prems" name1 by simp
+    next
+      case (BabTy_Array x81 x82 x83)
+      then show ?thesis using "1.prems" name1 by simp
+    qed
+  qed
+qed
+
+
+end
